\documentclass[a4paper,german,12pt,smallheadings]{scrartcl}
\usepackage[T1]{fontenc}
\usepackage[utf8]{inputenc}
\usepackage{babel}
\usepackage{tikz}
\usepackage{geometry}
\usepackage{amsmath}
\usepackage{amssymb}
\usepackage{float}
\usepackage{enumerate}
\usepackage{braket} % Teh quantum stuff
%\usepackage{wrapfig}
\usepackage[thinspace,thinqspace,squaren,textstyle]{SIunits}

% New command for color underlining
\usepackage{xcolor}

\newsavebox\MBox
\newcommand\colul[2][red]{{\sbox\MBox{$#2$}%
  \rlap{\usebox\MBox}\color{#1}\rule[-1.2\dp\MBox]{\wd\MBox}{0.5pt}}}

\restylefloat{table}
\geometry{a4paper, top=15mm, left=20mm, right=40mm, bottom=20mm, headsep=10mm, footskip=12mm}
\linespread{1.5}
\setlength\parindent{0pt}
\DeclareMathOperator{\Tr}{Tr}
\begin{document}
\begin{center}
\bfseries % Fettdruck einschalten
\sffamily % Serifenlose Schrift
\vspace{-40pt}
Quantum Mechanics, winter term 2013/2014, exercise sheet 4

Markus Fenske, Tutor: Adam Nagy
\vspace{-10pt}
\end{center}

\section*{Exercise 1: Uncertainty principle}
\begin{enumerate}[a)]
  \item
    When the electrons passes through a slit of width $d$, the uncertainty on the $x$-Axis is

    \begin{equation*}
      \Delta x = d
    \end{equation*}

    Therefore the uncertainty in momentum is
    \begin{equation*}
      \Delta p_x = \frac{\hbar}{2 \Delta x}
    \end{equation*}

    Using the non-relativistic momentum, we obtain for $\Delta v \ll v$

    \begin{equation*}
      \Delta p_x = \gamma m_e \Delta v_x
    \end{equation*}

    Therefore the uncertainty in speed is
    \begin{equation*}
      \Delta v_x = \frac{\hbar}{2 \gamma m_e \Delta x}
    \end{equation*}

    If the electrons need a time $t$ from the slit to the wall, the spatial uncertainty will be
    \begin{equation*}
      b = \Delta v_x \cdot t = \frac{\hbar}{2 \gamma m_e \Delta x} t
    \end{equation*}

    The time needed for a distance $d$ at speed $v$ is
    \begin{equation*}
      t = \frac{d}{v}
    \end{equation*}

    Using the relativistic equations for energy and momentum ($E_0 = mc^2$)
    \begin{equation*}
      E_\text{kin} = (\gamma - 1) E_0
    \end{equation*}

    We obtain
    \begin{equation*}
      v = c \sqrt{1- \frac{E_0^2}{(E_\text{kin} - E_0)^2}}
    \end{equation*}

    Therefore the complete equation is
    \begin{equation*}
      b = \frac{\hbar}{2 m_e \Delta x} \frac{d}{c \alpha} \sqrt{1 - \alpha},\qquad \alpha = \sqrt{1 - \frac{E_0^2}{(E_\text{kin} + E_0)^2}}
    \end{equation*}

    We get $\alpha \approx 0.4127$ ($v = 0.4127 c$) and therefore an additional beam width of
    \begin{equation*}
      b = 0.0251 \;\micro \meter
    \end{equation*}

    Therefore the total beam width should be
    \begin{equation*}
      w = 50 \pm 0.0251 \; \micro \meter
    \end{equation*}


  \item
    %\textbf{TODO:} Relativistic calculation, because of the huge energy.

    Using the uncertainty principle
    \begin{equation*}
      \Delta x \Delta p \ge \frac{\hbar}{2}
    \end{equation*}

    We get for the uncertainty of momentum:
    \begin{equation*}
      \Delta p \ge \frac{\hbar}{2 \Delta x}
    \end{equation*}

    The kinetic energy is
    \begin{equation*}
      E_\text{kin} = \frac{1}{2} mv^2 = \frac{p_0^2}{2m}
    \end{equation*}

    With the uncertain momentum $p_0 = p + \Delta p$ this leads to
    \begin{equation*}
      E_\text{kin} \ge \frac{(p + \frac{\hbar}{2 \Delta x})^2}{2m}
    \end{equation*}

    The minimal momentum is $p=0$, which results in the zero point energy
    \begin{equation*}
      E_\text{kin} \ge \frac{\hbar}{8 \Delta x^2 m}
    \end{equation*}

    With the given value of $\Delta x = 10^{-14} \; \meter$, this results in a
    minimum energy of $E_\text{kin,min} \approx 598 \; \mega\electronvolt$

  \item
    Using energy-time uncertainty
    \begin{equation*}
      \Delta E \Delta t \ge \frac{\hbar}{2}
    \end{equation*}

    And the photon energy
    \begin{equation*}
      E = h \nu
    \end{equation*}

    We obtain
    \begin{equation*}
      \Delta \nu \ge \frac{\hbar}{h} \frac{1}{2 \Delta t} = \frac{1}{4 \pi \Delta t}
    \end{equation*}

    For a pulse of $\Delta t = 1 \; \nano\second$ this results in a minium frequency width $\Delta \nu_\text{min}$ of
    \begin{equation*}
      \Delta \nu_\text{min} \approx 79.58 \; \mega\hertz
    \end{equation*}
  \item
    Using above equation with $\Delta t = 0.2 \; \second$, we obtain
    \begin{equation*}
      \Delta \nu_\text{min} \approx 0.398 \; \hertz
    \end{equation*}

    It would be easier to determine the frequency of a tone of higher pitch,
    because the percentual uncertainty is lower.
\end{enumerate}


\section*{Exercise 2: Fourier transformation}
(This part has been created in cooperation with Luis Herrmann and is identical)

\begin{enumerate}[a)]
\item \begin{align*}
&\hat{\psi}(k)=(\mathcal{F_\phi})(k)=c_1\int_{-\infty}^{\infty}\hat{\phi}(x)e^{ikx}dx\\
&\hat{\phi}(x)=(\mathcal{F^{-1}_\psi})(x)=c_2\int_{-\infty}^{\infty}\hat{\psi}(k)e^{-ikx}dk
\end{align*}
In order to determine the relation between integration constants $c_1$ and $c_2$, we insert our integral expression for $\hat{\psi}$ in $\hat{\phi}$:
\begin{align*}
\hat{\phi}(x)&=c_2\int_{-\infty}^{\infty}\left(c_1\int_{-\infty}^{\infty}\hat{\phi}(x)e^{ikx'}dx'\right)e^{-ikx}dk\\
&=c_2c_1\int_{-\infty}^{\infty}\left(\int_{-\infty}^{\infty}\hat{\phi}(x)e^{ikx'}dx'\right)e^{-ikx}dk
\end{align*}
This is an iterative integral. Generally, the order of integration of an iterative integral cannot lightheartedly be inverted, particularly not for improper integrals.\\

However, since we require both Fourier transformations to exist, the corresponding iterative integral over two variables must also exist and, according to Fubini's law, we can change the integration order. \\


Changing the order of integration:
\begin{equation*}
\hat{\phi}(x)=c_2c_1\int_{-\infty}^{\infty}\hat{\phi}(x')\left(\int_{-\infty}^{\infty}e^{ik(x'-x)}dk\right)dx'
\end{equation*}

The first integral is equivalent to the delta function:
\begin{equation*}
\int_{-\infty}^{\infty}e^{ik(x'-x)}=2\pi\delta(x-x')
\end{equation*}

Inserting this back into our main equation, we get:
\begin{equation*}
\hat{\phi}(x)=2\pi c_2c_1\int_{-\infty}^{\infty}\hat{\phi}(x')\delta(x-x')dx'
\end{equation*}

According to [http://mathworld.wolfram.com/DeltaFunction.html], the delta function has the fundamental property:
\begin{equation*}
\int_{- \infty}^{\infty}f(x')\delta(x-x')dx'=f(x)
\end{equation*}

This will also apply for $\hat{\phi}(x)$ and we obtain the following relation:
\begin{align*}
&\hat{\phi}(x)=2\pi c_2c_1\hat{\phi}(x)\\
\Leftrightarrow & c_1c_2=\frac{1}{2\pi}
\end{align*}

\item

The $\mathcal{L}^2$ scalar product is defined as:
\begin{equation*}
\braket{\psi\,\phi}=\int\overline{\psi}(x)\phi(x)dx
\end{equation*}
Let:
\begin{equation*}
\mathcal{F}_{\psi}(k)=c_1\int_{-\infty}^{\infty}e^{-ikx}\psi(x)dx \quad \text{and} \quad \mathcal{F}_{\phi}(k)=c_1\int_{-\infty}^{\infty}e^{-ikx}\phi(x)dx
\end{equation*}
We require the Fourier transformation to be unitarian, such that:
\begin{equation*}
\braket{\psi,\phi}=\braket{\mathcal{F}_{\psi},\mathcal{F}_{\phi}}
\end{equation*}
... is fulfilled. Let us consider the $\mathcal{L}^2$ scalar product of the Fourier transformations:
\begin{align*}
\braket{\mathcal{F}_{\psi},\mathcal{F}_{\phi}}&=\int_{-\infty}^{\infty}\overline{\mathcal{F}_{\psi}(k)}\mathcal{F}_{\phi}(k)dk\\
&=\int_{-\infty}^{\infty}\left(\overline{c_1\int_{-\infty}^{\infty}e^{-ikx}\psi(x)dx}\right)\left(c_1\int_{-\infty}^{\infty}e^{-ikx'}\phi(x')dx'\right)dk\\
&=\overline{c_1}c_1\int_{-\infty}^{\infty}\left(\int_{-\infty}^{\infty}e^{ikx}\overline{\psi(x)}dx\right)\left(\int_{-\infty}^{\infty}e^{-ikx'}\phi(x')dx'\right)dk
\end{align*}
Applying the same argumentation as for (a), we may change the order of integration:
\begin{equation*}
\braket{\mathcal{F}_{\psi},\mathcal{F}_{\phi}}=\overline{c_1}c_1\int_{-\infty}^{\infty}\left(\int_{-\infty}^{\infty}\overline{\psi(x)}\phi(x')\right)\left(\int_{-\infty}^{\infty}e^{ik(x-x')}\right)dkdxdx'
\end{equation*}
Again, the first iteration of the integral is equivalent to $2\pi$ times the delta function and we get:
\begin{align*}
\braket{\mathcal{F}_{\psi},\mathcal{F}_{\phi}}&=2\pi\overline{c_1}c_1\int_{-\infty}^{\infty}\int_{-\infty}^{\infty}\overline{\psi(x)}\phi(x')\delta(x-x')dxdx'\\
&=2\pi \overline{c_1}c_1\int_{-\infty}^{\infty}\overline{\psi(x)}\phi(x)dx \quad \text{()see above}\\
&=2\pi\overline{c_1}c_1\braket{\psi,\phi}\\
&=2\pi|c_1|^2\braket{\psi,\phi} \quad \quad \text{since} \quad \overline{c_1}c_1=|c_1|^2 \quad \forall c_1\in\mathbb{C}
\end{align*}

Using our initial condition of the scalar product being unitarian, we finally obtain:
\begin{align*}
&\braket{x,y}=\braket{\mathcal{F}_{\psi},\mathcal{F}_{\phi}}\\
\Leftrightarrow \quad &\braket{\psi,\phi}=2\pi|c_1|^2\braket{\psi,\phi}\\
\Leftrightarrow \quad &|c_1|=\frac{1}{\sqrt{2\pi}}
\end{align*}

Thus, using our results from (a), the inverse transformation constant must be:
\begin{equation*}
|c_2|=\frac{1}{2\pi |c_1|} \quad \Leftrightarrow \quad |c_2|=\frac{1}{\sqrt{2\pi}}
\end{equation*}

\end{enumerate}

\section*{Exercise 3: Commutators and eigenvalues of hermitian $2 \times 2$ matricies}
\begin{enumerate}[a)]
  \item
    (i)
    \begin{align*}
      &[A, BC] =
      ABC - BCA =
      ABC - BCA + (BAC-BAC) =
      BAC - BCA + ABC - BAC = \\
      &B(AC-CA) + (AB-BA)C =
      B[A,C] + [A,B]C
    \end{align*}
    (ii)
    \begin{align*}
      &[A, [B,C]] + [B, [C,A]] + [C, [A,B]] = \\
      &[A, (BC-CB)] + [B, (CA-AC)] + [C, (AB-BA)] = \\
      &A(BC-CB)-(BC-CB)A + B(CA-AC)-(CA-AC)B + C(AB-BA)-(AB-BA)C = \\
      &\colul[red]{ABC}\colul[green]{-ACB}\colul[blue]{-BCA}\colul[yellow]{+CBA} \;\;
      \colul[blue]{+BCA}\colul[magenta]{-BAC}\colul[cyan]{-CAB}\colul[green]{+ACB} \;\;
      \colul[cyan]{+ CAB}\colul[yellow]{-CBA}\colul[red]{-ABC}\colul[magenta]{+BAC} = 0
    \end{align*}
  \item
    Determinant:
    \begin{equation*}
      \det M = \alpha\beta - \gamma\gamma^* = \alpha\beta - |\gamma|^2
    \end{equation*}

    Trace:
    \begin{equation*}
      \operatorname{tr} M = \alpha\beta
    \end{equation*}

    Eigenvalues:
    \begin{align*}
      &\det(M-\lambda I) = (\alpha - \lambda)(\beta - \lambda) - |\gamma|^2 \overset{!}{=} 0 \\
      \Leftrightarrow\quad& \alpha\beta - \alpha\lambda - \beta\lambda + \lambda^2 - |\gamma|^2 = 0 \\
      \Leftrightarrow\quad& \lambda^2 - \lambda(\alpha + \beta) - |\gamma|^2 + \alpha\beta = 0 \\
      \Leftrightarrow\quad& \lambda_{1,2} = \frac{\alpha+\beta}{2} \pm \sqrt{\frac{(\alpha + \beta)^2}{4} + |\gamma|^2 - \alpha\beta} \\
      & \quad\;\;\, = \frac{\alpha+\beta}{2} \pm \sqrt{\frac{\alpha^2 + 2\alpha\beta + \beta^2}{4} + |\gamma|^2 - \alpha\beta} \\
      & \quad\;\;\, = \frac{\alpha+\beta}{2} \pm \sqrt{\frac{\alpha^2 - 2\alpha\beta + \beta^2}{4} + |\gamma|^2} \\
      & \quad\;\;\,= \frac{\alpha+\beta}{2} \pm \sqrt{\frac{(\alpha - \beta)^2}{4} + |\gamma|^2} \\
    \end{align*}

    The term under the square root is $\ge 0$, because $\alpha, \beta,
    |\gamma|$ are real numbers. So the eigenvalues must be real numbers.
\end{enumerate}

\section*{Exercise 4: Pauli matricies}
\begin{enumerate}[a)]
  \item
    Traces:
    \begin{equation*}
      \operatorname{tr} \sigma_0 = 1, \qquad
      \operatorname{tr} \sigma_1 = 0, \qquad
      \operatorname{tr} \sigma_2 = 0, \qquad
      \operatorname{tr} \sigma_3 = 0
    \end{equation*}

    Determinants:
    \begin{equation*}
      \det \sigma_0 = 0, \qquad
      \det \sigma_1 = -1, \qquad
      \det \sigma_2 = -1, \qquad
      \det \sigma_1 = -1
    \end{equation*}

    Eigenvalues (using the formula from 3b):
    \begin{equation*}
      \lambda_{\sigma_0} = \{1,1\}, \qquad
      \lambda_{\sigma_1} = \{-1,1\}, \qquad
      \lambda_{\sigma_2} = \{-1,1\}, \qquad
      \lambda_{\sigma_3} = \{-1,1\}
    \end{equation*}

    The matricies are obviously hermitian (because $\sigma_n = \sigma_n^\dagger$).
  \item
    \begin{align*}
      \delta_{12} = 0, \epsilon_{123} = 1 \qquad\Rightarrow\qquad
      &\sigma_1\sigma_2 =
      \begin{pmatrix} 0 & 1 \\ 1 & 0 \end{pmatrix}
      \begin{pmatrix} 0 & -i \\ i & 0 \end{pmatrix}
      =
      \begin{pmatrix} i & 0 \\ 0 & -i \end{pmatrix} = i\sigma_3 \\
      \delta_{23} = 0, \epsilon_{231} = 1 \qquad\Rightarrow\qquad
      &\sigma_2\sigma_3 =
      \begin{pmatrix} 0 & -i \\ i & 0 \end{pmatrix}
      \begin{pmatrix} 1 & 0 \\ 0 & -1\end{pmatrix}
      =
      \begin{pmatrix} 0 & i \\ i & 0\end{pmatrix} = i\sigma_1 \\
      \delta_{23} = 0, \epsilon_{132} = -1 \qquad\Rightarrow\qquad
      &\sigma_1\sigma_3 =
      \begin{pmatrix} 0 & 1 \\ 1 & 0 \end{pmatrix}
      \begin{pmatrix} 1 & 0 \\ 0 & -1\end{pmatrix}
      =
      \begin{pmatrix} 0 & -1 \\ 1 & 0\end{pmatrix}
      = -i\sigma_2
    \end{align*}

    Using the given equation:

    \begin{equation*}
      [\sigma_i, \sigma_j] = \sigma_i\sigma_j - \sigma_j\sigma_i =
      \delta_{ij}\sigma_0 + i \sum_{k=1}^3 \epsilon_{ijk} \sigma_k -
      \left(\delta_{ji}\sigma_0 + i \sum_{k=1}^3 \epsilon_{jik} \sigma_k\right)
    \end{equation*}

    \textbf{Case 1:} For $i \neq j$, the Kronecker deltas will vanish.  Because $\epsilon_{ijk}
    = -\epsilon_{jik}$, this leads to

    \begin{equation*}
      [\sigma_i, \sigma_j] = 2i \sum_{k=1}^3 \epsilon_{ijk} \sigma_k
    \end{equation*}

    \textbf{Case 2:} If $i=j$, the commutator will be $[\sigma_i, \sigma_i] =
    0$, therefore the sum should vanish. The Levi-Civita symbol will
    become $\epsilon_{iik} = 0$. Therefore the equation is true for $i = j$ as
    well.
  \item
    To prove orthogonality, we have to prove that
    \begin{equation*}
      \braket{\sigma_i, \sigma_j} = 0 \; \forall i \neq j
    \end{equation*}

    Given $i=0, j \in {1,2,3}$ it's obvious that the scalar product vanishes,
    because $\braket{\sigma_0, \sigma_j} = \Tr \sigma_j = 0$.

    If $i \neq 0$ then
    \begin{equation*}
      \braket{\sigma_i, \sigma_j} = \Tr(\sigma_i \sigma_j) = \Tr(i \sum_{k=1}^3 \epsilon_{ijk} \sigma_k) = i \Tr(\sigma_k)
    \end{equation*}
    Because the trace of all Pauli matrices vanishes it is $\Tr \sigma_k = 0$

    Therefore all Pauli matricies are orthogonal.

    To calculate the $c_i$, we just need to solve the system of linear equations.

    \begin{equation*}
    M = \sum_{i=0}^3 c_i \sigma_i
    \end{equation*}

    This can be written as:
    \begin{equation*}
      \begin{pmatrix}
        \alpha & \beta \\ \gamma & \delta
      \end{pmatrix}
      =
      c_0
      \begin{pmatrix}
        1 & 0 \\
        0 & 1
      \end{pmatrix}
      +
      c_1
      \begin{pmatrix}
        0 & 1 \\
        1 & 0
      \end{pmatrix}
      +
      c_2
      \begin{pmatrix}
        0 & -i \\
        i & 0
      \end{pmatrix}
      +
      c_3
      \begin{pmatrix}
        1 & 0 \\
        0 & -1
      \end{pmatrix}
    \end{equation*}

    Which is can be solved to
    \begin{equation*}
      c_0 = \frac{\alpha + \delta}{2}, \qquad
      c_1 = \frac{\beta + i \gamma}{2}, \qquad
      c_2 = \frac{\beta - i \gamma}{2}, \qquad
      c_3 = \frac{\alpha - \delta}{2}
    \end{equation*}

\end{enumerate}

\end{document}
